### Exercice 34

On utilise la formule : $(g(ax+b))'=a\times g'(ax+b)$


1. $f(x) = \mathrm e^{3x} = \mathrm e^{3\times x + 0}$, donc
$f'(x) = 3 \times \mathrm e^{3\times x + 0}$, $f'$ est strictement  positive sur $\mathbb R$, donc $f$ est strictement  croissante sur $\mathbb R$.

2. $f(x)=\mathrm e^{-2x}$, donc $f'(x) = -2 \times \mathrm e^{-2x}$, $f'$ est strictement négative sur $\mathbb R$, donc $f$ est strictement  décroissante sur $\mathbb R$.


3. $f(x)=\mathrm e^{-x+4}$, donc $f'(x) = -1 \times \mathrm e^{-x+4}$, $f'$ est strictement négative sur $\mathbb R$, donc $f$ est strictement  décroissante sur $\mathbb R$.


4. $f(x) = 5\mathrm e^{x+6} = 5\mathrm e^{1\times x + 6}$, donc
$f'(x) = 5 \times 1 \times \mathrm e^{1\times x + 6}$, $f'$ est strictement  positive sur $\mathbb R$, donc $f$ est strictement  croissante sur $\mathbb R$.


