### Exercice 59

Quelques formules utiles de calcul litt√©ral :
* $(a+b)^2 = a^2 +2ab + b^2$
* $(a-b)^2 = a^2 -2ab + b^2$
* $(a-b)(a+b) = a^2 - b^2$


1. Calcul de $D$
$D(x) = \left( \mathrm e^{x} + \mathrm e^{-2x}  \right)^2$
$D(x) = \left(\mathrm e^{x}\right)^2 +2\mathrm e^{x}\times\mathrm e^{-2x}  + \left(\mathrm e^{-2x}\right)^2$
$D(x) = \mathrm e^{2x} +2\mathrm e^{x-2x}  + \mathrm e^{-4x}$
$D(x) = \mathrm e^{2x} +2\mathrm e^{-x}  + \mathrm e^{-4x}$.

2. Calcul de $E$
$E(x) = \left( \mathrm e^{3x} - \mathrm e^{5x}  \right)^2$
$E(x) = \left(\mathrm e^{3x}\right)^2 -2\mathrm e^{3x}\times\mathrm e^{5x}  + \left(\mathrm e^{5x}\right)^2$
$E(x) = \mathrm e^{6x} -2\mathrm e^{3x+5x}  + \mathrm e^{10x}$
$E(x) = \mathrm e^{6x} -2\mathrm e^{8x}  + \mathrm e^{10x}$.

3. Calcul de $F$
$F(x) = \left( \mathrm e^{-2x} - \mathrm e^{x}  \right) \left( \mathrm e^{-2x} + \mathrm e^{x}  \right)$
$F(x) = \left(\mathrm e^{-2x}\right)^2 - \left(\mathrm e^{x}\right)^2$
$F(x) = \mathrm e^{-4x} - \mathrm e^{2x}$.

