# Exercice 70 p 174

DÃ©river et factoriser

Avec la formule

$$(uv)' = u'v + uv'$$

1. \
    **$f(x) = (x+1)\mathrm e^x$**
    $f'(x) = 1\times \mathrm e^x + (x+1)\mathrm e^x$
    $f'(x) = \left(1+ (x+1)\right)\mathrm e^x$
    $f'(x) = (x+2)\mathrm e^x$
2. \
    **$f(x) = (-2x+3)\mathrm e^x$**
    $f'(x) = -2\times \mathrm e^x + (-2x+3)\mathrm e^x$
    $f'(x) = \left(-2+ (-2x+3)\right)\mathrm e^x$
    $f'(x) = (-2x+1)\mathrm e^x$
3. \
    **$f(x) = x^2\mathrm e^x$**
    $f'(x) = 2x\times \mathrm e^x + x^2\mathrm e^x$
    $f'(x) = \left(2x+x^2\right)\mathrm e^x$
    $f'(x) = x(x+2)\mathrm e^x$
4. \
    **$f(x) = (x^2-3x+1)\mathrm e^x$**
    $f'(x) = (2x-3)\times \mathrm e^x + (x^2-3x+1)\mathrm e^x$
    $f'(x) = \left((2x-3)+ (x^2-3x+1)\right)\mathrm e^x$
    $f'(x) = (x^2-x-2)\mathrm e^x$ ; on peut encore factoriser avec $\Delta = (-1)^2 - 4\times1\times(-2)= 9 > 0$
    $f'(x) = (x+1)(x-2)\mathrm e^x$
